Makefile
@@ -65,7 +65,9 @@ tmonad-gen: insert/insert_log_gen.v \
             make_array/make_array_linear_gen.v \
             sub1/sub1_gen.v \
             sub1/sub1_linear_loop_gen.v \
-            fold/fold_gen.v
+            fold/fold_gen.v \
+            clrs/insert_gen.v \
+            clrs/isort_gen.v
 
 insert/insert_log_gen.v: rkt/insert.rkt $(GEN_DEPS)
 	racket rkt/insert.rkt > insert/insert_log_gen.v
@@ -121,6 +123,11 @@ sub1/sub1_linear_loop_gen.v: rkt/sub1_linear_loop.rkt $(GEN_DEPS)
 	racket rkt/sub1_linear_loop.rkt > sub1/sub1_linear_loop_gen.v
 fold/fold_gen.v: rkt/fold.rkt $(GEN_DEPS)
 	racket rkt/fold.rkt > fold/fold_gen.v
+
+clrs/insert_gen.v: rkt/isort_insert.rkt $(GEN_DEPS)
+	racket rkt/isort_insert.rkt > clrs/insert_gen.v
+clrs/isort_gen.v: rkt/isort.rkt $(GEN_DEPS)
+	racket rkt/isort.rkt > clrs/isort_gen.v
 
 Makefile.coq: tmonad-gen Makefile $(VS)
 	coq_makefile -R . Braun $(VS) -o Makefile.coq
